ha2_refl.v
@@ -2,11 +2,7 @@
 
 Require Import ha2.
 
-Locate "≃".
-
 Require Import Arith.
-
-Search Nat.ltb.
 
 Fixpoint closed_tm (level : fin) (t : tm) : bool :=
   match t with
@@ -36,8 +32,6 @@ Notation "t ≄ u" := ((t ≃ u) ⇒ ⊥)(at level 20).
 Locate "∃".
 
 Import ListNotations.
-
-Check is_true.
 
 Coercion is_true : bool >-> Sortclass.
 
@@ -223,32 +217,85 @@ Proof.
       apply (fun _ _ => False).
 Qed.
 
+Require Import Lia.
+
+Lemma lower_closed : forall t level, closed_tm 0 t -> lower_tm level t = Some t.
+Proof.
+  induction t; simpl; intros; try congruence.
+  - destruct (Nat.ltb_spec n 0); try lia; congruence.
+  - rewrite IHt; simpl; auto.
+  - unfold is_true in *.
+    rewrite Bool.andb_true_iff in H.
+    rewrite IHt1, IHt2; simpl; intuition.
+  - unfold is_true in *.
+    rewrite Bool.andb_true_iff in H.
+    rewrite IHt1, IHt2; simpl; intuition.
+Qed.
+
+Lemma match_closed : forall level t, closed_tm 0 t -> match_var level level t = Success t.
+  unfold match_var.
+  intros.
+  destruct (Nat.ltb_spec level level); try lia.
+  destruct (Nat.eqb_spec level level); try lia.
+  rewrite lower_closed; auto.
+Qed.
+
+Lemma match_closed' : forall level n t, closed_tm 0 t -> level <> n -> match_var level n t = Fail.
+  unfold match_var.
+  intros.
+  destruct (Nat.ltb_spec n level).
+  - destruct t; simpl in *; auto.
+    unfold is_true in *; rewrite Nat.ltb_lt in H; lia.
+  - destruct (Nat.eqb_spec n level); try lia.
+    destruct t; try congruence.
+    simpl in H.
+    unfold is_true in *; rewrite Nat.ltb_lt in H; lia.
+Qed.
+
+Lemma match_closed_tm : forall t level, closed_tm 0 t -> match_tm level t t = Empty.
+Proof.
+  induction t; simpl; auto.
+  - intros ?; destruct (Nat.ltb_spec n 0); [lia | congruence].
+  - intros level; unfold is_true; rewrite Bool.andb_true_iff; intros (h1 & h2);
+      rewrite IHt1, IHt2; intuition.
+  - intros level; unfold is_true; rewrite Bool.andb_true_iff; intros (h1 & h2);
+      rewrite IHt1, IHt2; intuition.
+Qed.
+    
+
+Require Import Coq.Classes.EquivDec.
+
 
 Lemma neq_closed : forall n m Γ, n <> m -> Γ ⊢ n_tm n ≄ n_tm m.
 Proof.
   induction n; induction m; simpl; intros; try congruence.
   - apply imp_intro.
     apply imp_elim with (P := (Succ (n_tm m) ≃ Z)).
-    + replace (Succ (n_tm m) ≄ Z) with (Succ (var_tm 0) ≄ Z)[(n_tm m)..;ids] by (asimpl; auto).
-      apply forallt_elim.
-      apply zero_S.
+    + eapply apply_forallt; [| apply zero_S; eauto].
+      simpl; rewrite match_closed; auto.
+      reflexivity.
     + apply sym_apply.
       apply (axiom 0); auto.
-  - replace (Succ (n_tm n) ≄ Z) with (Succ (var_tm 0) ≄ Z)[(n_tm n)..;ids] by (asimpl; auto).
-    apply forallt_elim.
-    apply zero_S.
+  - eapply apply_forallt; [ | apply zero_S; eauto].
+    simpl; rewrite match_closed; auto; reflexivity.
   - apply imp_intro.
     apply imp_elim with (P := (n_tm n) ≃ (n_tm m)).
     + apply IHn; auto.
     + eapply imp_elim; [| apply (axiom 0); simpl; eauto].
-      Check inj_S.
-      replace (Succ (n_tm n) ≃ Succ (n_tm m) ⇒ n_tm n ≃ n_tm m)
-        with (Succ (n_tm n) ≃ Succ (var_tm 0) ⇒ n_tm n ≃ var_tm 0)[(n_tm m)..; ids]
-        by (asimpl; rewrite subst_closed; auto).
-      apply forallt_elim.
-      replace (all Succ (n_tm n) ≃ Succ (var_tm 0) ⇒ n_tm n ≃ var_tm 0) with (all Succ (var_tm 1) ≃ Succ (var_tm 0) ⇒ var_tm 1 ≃ var_tm 0)[(n_tm n)..; ids] by (asimpl; rewrite ren_closed; auto).
-      apply forallt_elim.
-      apply inj_S.
+      eapply apply_forallt2 with (t1 := (n_tm n)); [ | | apply inj_S].
+      -- simpl; rewrite match_closed; [ | asimpl; rewrite ren_closed; auto].
+         asimpl.
+         unfold match_var; simpl.
+         rewrite ren_closed; auto.
+         unfold join.
+         rewrite eq_dec_eq.
+         auto.
+      -- simpl; rewrite match_closed; auto.
+         rewrite ren_closed; auto.
+         asimpl.
+         rewrite match_closed_tm; auto.
+         unfold join.
+         rewrite eq_dec_eq; eauto.
 Qed.
 
 
@@ -310,18 +357,21 @@ Proof.
        unfold idsRen;
        asimpl;
         rewrite subst_lift'; auto).
-  apply forallt_elim.
-  
+  apply forallt_elim.  
   replace (all var_tm 0 ∈ {{_ | P ⟨↑ >> ↑ ; ids⟩ }}) with
     (all var_tm 0 ∈ var_pred 0)[ids; {{_ | P ⟨↑ ; ids⟩ }}..] by (asimpl; auto).
   apply forallP_elim; auto.
 Qed.
 
-Notation "P ∧ Q" := (FORALL (P⟨id; ↑⟩ ⇒ Q⟨id; ↑⟩ ⇒ all (var_tm 0) ∈ (var_pred 0)) ⇒ all (var_tm 0) ∈ (var_pred 0)) (at level 25).
+Definition and_prop P Q := FORALL (P⟨id; ↑⟩ ⇒ Q⟨id; ↑⟩ ⇒ all (var_tm 0) ∈ (var_pred 0)) ⇒ all (var_tm 0) ∈ (var_pred 0).
 
-Notation "P ∨ Q" := (FORALL (P⟨id; ↑⟩ ⇒ all (var_tm 0) ∈ (var_pred 0)) ⇒
+Notation "P ∧ Q" := (and_prop P Q) (at level 25).
+
+Definition or_prop P Q := FORALL (P⟨id; ↑⟩ ⇒ all (var_tm 0) ∈ (var_pred 0)) ⇒
                             (Q⟨id; ↑⟩ ⇒ all (var_tm 0) ∈ (var_pred 0)) ⇒
-                            all (var_tm 0) ∈ (var_pred 0)) (at level 25).
+                            all (var_tm 0) ∈ (var_pred 0).
+
+Notation "P ∨ Q" := (or_prop P Q) (at level 25).
 
 
 Class complete Γ P := { reflect : Γ ⊧ P -> Γ ⊢ P }.
@@ -370,14 +420,17 @@ Print "⊧".
 Definition bot_pval : PVal := fun _ _ => False.
 Definition bot_vval : VVal := fun _ => 0.
 
+Lemma val_nil : validates bot_pval bot_vval nil.
+Proof.
+  unfold validates; auto.
+Qed.
+
 Theorem ex_refl :
   forall P, [] ⊢ ∃ P -> exists n, eval_prop bot_pval (n, bot_vval) P.
 Proof.
   intros.
-  Check soundness.
   assert (h : [] ⊧ ∃ P) by (apply soundness; auto).
   unfold "⊧" in *; simpl in *.
-  assert (val_nil : validates bot_pval bot_vval nil) by (unfold validates; auto).
   apply (h bot_pval bot_vval val_nil (fun _ => exists n, eval_prop bot_pval (n, bot_vval) P)); [ | exact 0].
   intros.
   exists n.
@@ -385,20 +438,217 @@ Proof.
   auto.
 Qed.
 
+(* Todo: prove that there actually is a *provable* inhabitant! (at least when we're Deta_0) *)
+                   
 Theorem and_intro : forall Γ P Q, Γ ⊢ P ⇒ Q ⇒ P ∧ Q.
-Abort.
+  intros.
+  repeat apply imp_intro.
+  apply forallP_intro.
+  repeat apply imp_intro.
+  eapply imp_elim with (P := Q ⟨id;↑⟩).
+  - eapply imp_elim with (P := P ⟨id;↑⟩); [apply (axiom 0); auto |].
+    apply (axiom 2); auto.
+  - apply (axiom 1); auto.
+Qed.
+
+Lemma sheesh : forall (P : prop) ξ, P [ξ >> var_tm; var_pred] = P ⟨ξ; id⟩.
+Proof.
+  induction P using prop_pred_ind with (P0 :=  fun P => forall ξ, P [ξ >> var_tm; var_pred] = P ⟨ξ; id⟩); simpl; asimpl; try rewrite IHP; auto.
+  - intros; rewrite subst_ren; rewrite IHP; asimpl; auto.
+  - intros.
+    rewrite ext_prop with (tautm := (0, ξ >> S) >> var_tm)(taupred := var_pred).
+    + rewrite IHP; auto.
+    + destruct x; asimpl; auto.
+    + auto.
+  - intros; rewrite ext_prop with (tautm := ξ >> var_tm)(taupred := var_pred); auto.
+    rewrite IHP.
+    rewrite extRen_prop with (zetatm := ξ)(zetapred := (0, S)); auto.
+    destruct x; auto.
+  - intros; rewrite IHP1, IHP2; auto.
+  - intros.
+    rewrite ext_prop with (tautm := (0, ξ >> S) >> var_tm)(taupred := var_pred); auto.
+    + rewrite IHP; auto.
+    + destruct x; asimpl; auto.
+Qed.
 
 Theorem and_elim1 : forall Γ P Q, Γ ⊢ P ∧ Q ⇒ P.
-Abort.
+Proof.                     
+  intros; repeat apply imp_intro.
+  unfold "∧".
+  replace P with P⟨↑; id⟩[(var_tm 0)..; ids] at 2 by (asimpl; auto).
+  apply compr_elim.
+  pattac (var_tm 0).
+  apply forallt_elim.
+  simpl; asimpl.
+  apply imp_elim with (P := P ⇒ Q ⇒ (all var_tm 0 ∈ {{ _ | P⟨↑ >> S ; id⟩}})).
+  - pose (Pu := P ⟨↑ >> S; id⟩).
+    replace (P ⟨↑ >> S; id⟩) with Pu by reflexivity.
+    replace (ren_prop (↑ >> S) id P) with Pu by reflexivity.
+    replace ((P ⇒ Q ⇒ (all var_tm 0 ∈ ({{ _ | Pu }}))) ⇒ (all var_tm 0 ∈ ({{ _ | Pu }})))
+      with
+      ((P⟨id;↑⟩ ⇒ Q ⟨id;↑⟩ ⇒ (all var_tm 0 ∈ var_pred 0)) ⇒ (all var_tm 0 ∈ var_pred 0))[ids; {{ _ | P⟨↑;id⟩ }}..] by (subst Pu; asimpl; auto).
+    apply forallP_elim.
+    apply (axiom 0); auto.
+  - repeat apply imp_intro.
+    apply forallt_intro.
+    apply compr_intro.
+    apply (axiom 1); asimpl; simpl.
+    replace (P ⟨↑; id⟩) with (subst_prop (↑ >> var_tm) var_pred P); auto.
+    
+    replace (subst_prop (↑ >> var_tm) var_pred P) with (P ⟨↑; id⟩[var_tm; var_pred]) ; (asimpl; auto).
+    rewrite sheesh; auto.
+Qed.
 
 Theorem and_elim2 : forall Γ P Q, Γ ⊢ P ∧ Q ⇒ Q.
-Abort.
+Proof.                     
+  intros; repeat apply imp_intro.
+  unfold "∧".
+  replace Q with Q⟨↑; id⟩[(var_tm 0)..; ids] at 2 by (asimpl; auto).
+  apply compr_elim.
+  pattac (var_tm 0).
+  apply forallt_elim.
+  simpl; asimpl.
+  apply imp_elim with (P := P ⇒ Q ⇒ (all var_tm 0 ∈ {{ _ | Q⟨↑ >> S ; id⟩}})).
+  - pose (Qu := Q ⟨↑ >> S; id⟩).
+    replace (Q ⟨↑ >> S; id⟩) with Qu by reflexivity.
+    replace (ren_prop (↑ >> S) id Q) with Qu by reflexivity.
+    replace ((P ⇒ Q ⇒ (all var_tm 0 ∈ ({{ _ | Qu }}))) ⇒ (all var_tm 0 ∈ ({{ _ | Qu }})))
+      with
+      ((P⟨id;↑⟩ ⇒ Q ⟨id;↑⟩ ⇒ (all var_tm 0 ∈ var_pred 0)) ⇒ (all var_tm 0 ∈ var_pred 0))[ids; {{ _ | Q⟨↑;id⟩ }}..] by (subst Qu; asimpl; auto).
+    apply forallP_elim.
+    apply (axiom 0); auto.
+  - repeat apply imp_intro.
+    apply forallt_intro.
+    apply compr_intro.
+    apply (axiom 0); asimpl; simpl.
+    replace (Q ⟨↑; id⟩) with (subst_prop (↑ >> var_tm) var_pred Q); auto.
+    
+    replace (subst_prop (↑ >> var_tm) var_pred Q) with (Q ⟨↑; id⟩[var_tm; var_pred]) ; (asimpl; auto).
+    rewrite sheesh; auto.
+Qed.
 
 Theorem or_intro1 : forall Γ P Q, Γ ⊢ P ⇒ P ∨ Q.
-Abort.
+Proof.
+  intros; repeat apply imp_intro.
+  unfold "∨".
+  apply forallP_intro.
+  repeat apply imp_intro.
+  eapply imp_elim; [apply (axiom 1); simpl; eauto | ].
+  apply (axiom 2); simpl; auto.
+Qed.
 
 Theorem or_intro2 : forall Γ P Q, Γ ⊢ Q ⇒ P ∨ Q.
-Abort.
+Proof.
+  intros; repeat apply imp_intro.
+  unfold "∨".
+  apply forallP_intro.
+  repeat apply imp_intro.
+  eapply imp_elim; [apply (axiom 0); simpl; eauto | ].
+  apply (axiom 2); simpl; auto.
+Qed.
+
 
 Theorem or_elim : forall Γ P Q R, Γ ⊢ P ⇒ R -> Γ ⊢ Q ⇒ R -> Γ ⊢ P ∨ Q ⇒ R.
-Abort.
+Proof.
+  intros; repeat apply imp_intro.
+  unfold "∨".
+  replace R with (R⟨↑; id⟩[(var_tm 0)..; ids]) by (asimpl; auto).
+  apply compr_elim.
+  pattac (var_tm 0).  
+  apply forallt_elim.
+  simpl; asimpl.
+  pose (R' := {{_ | ren_prop (↑ >> S) id R}}).
+  replace ({{_ | ren_prop (↑ >> S) id R}}) with R' by auto.
+  apply imp_elim with (P := Q ⇒ (all var_tm 0 ∈ R')).
+  - apply imp_elim with (P := P ⇒ (all var_tm 0 ∈ R')).
+    + replace ((P ⇒ (all var_tm 0 ∈ R')) ⇒ (Q ⇒ (all var_tm 0 ∈ R')) ⇒ (all var_tm 0 ∈ R'))
+        with ((P⟨id; ↑⟩ ⇒ (all var_tm 0 ∈ var_pred 0)) ⇒ (Q⟨id; ↑⟩ ⇒ (all var_tm 0 ∈ var_pred 0)) ⇒ (all var_tm 0 ∈ var_pred 0))[ids; {{ _ | R⟨↑; id⟩}}..] by (asimpl; auto).
+      apply forallP_elim; apply (axiom 0); auto.
+    + apply imp_intro, forallt_intro, compr_intro.
+      asimpl.
+      rewrite sheesh.
+      eapply imp_elim; [ | apply (axiom 0); simpl; auto].
+      unfold lift_tm; simpl.
+      apply weakening.
+      apply weakening.
+      replace (P ⟨↑;id⟩ ⇒ R ⟨↑;id⟩) with (P ⇒ R)⟨↑; id⟩ by (asimpl; auto).
+      apply lift_derives; auto.
+  -  apply imp_intro, forallt_intro, compr_intro.
+      asimpl.
+      rewrite sheesh.
+      eapply imp_elim; [ | apply (axiom 0); simpl; auto].
+      unfold lift_tm; simpl.
+      apply weakening.
+      apply weakening.
+      replace (Q ⟨↑;id⟩ ⇒ R ⟨↑;id⟩) with (Q ⇒ R)⟨↑; id⟩ by (asimpl; auto).
+      apply lift_derives; auto.
+Qed.
+
+(* TODO: completeness for ∨ and ∧ *)
+Instance and_complete {P Q}{cpltP : complete nil P}{cpltQ : complete nil Q} : complete nil (P ∧ Q).
+Proof.
+  constructor.
+  destruct cpltP, cpltQ.
+  intros.
+  eapply imp_elim; [| apply reflect1].
+  eapply imp_elim; [| apply reflect0].
+  - apply and_intro.
+  - unfold "∧" in H.
+    unfold models in H.
+    simpl in H.
+    intro; intros.
+    apply (H pval vval); eauto; [| exact 0].
+    rewrite eval_ren; asimpl.
+    auto.
+  - unfold "∧" in H.
+    unfold models in H.
+    simpl in H.
+    intro; intros.
+    apply (H pval vval); eauto; [| exact 0].
+    intros _; rewrite eval_ren; asimpl.
+    auto.
+Qed.
+
+Lemma closed_eval_tm : forall t vval vval',
+ closed_tm 0 t -> eval_tm vval t = eval_tm vval' t.
+Proof.
+  induction t; simpl; intros; unfold is_true in *; auto.
+  - rewrite Nat.ltb_lt in *; lia.
+  - rewrite Bool.andb_true_iff in *; intuition.
+  - rewrite Bool.andb_true_iff in *; intuition.
+Qed.
+
+
+Lemma closed_eval : forall P vval pval vval' pval',
+ closed_prop 0 0 P -> eval_prop pval vval P <-> eval_prop pval' vval' P.
+Proof.
+  induction P using prop_pred_ind
+    with (P0 := fun p => forall vval pval vval' pval', closed_pred 0 0 p -> forall n, eval_pred pval vval p n <-> eval_pred pval' vval' p n); simpl; unfold is_true; intros; auto.
+  - rewrite Bool.andb_true_iff in *; erewrite closed_eval_tm; try apply IHP; intuition.
+  - admit.
+  - admit.
+  - rewrite Bool.andb_true_iff in *.
+    rewrite IHP1, IHP2; [reflexivity | |]; intuition.
+  - rewrite Nat.ltb_lt in *; lia.
+  - admit.
+Admitted.
+
+(* is this even true? Certainly if P and Q are closed... *)
+Instance or_complete {P Q}{cpltP : complete nil P}{cpltQ : complete nil Q} : closed_prop 0 0 P -> closed_prop 0 0 Q -> complete nil (P ∨ Q).
+Proof.
+  intros clp clq; constructor; destruct cpltP, cpltQ; unfold models; simpl; intros h.
+  (* Unclear that this holds! what if P is is_even n and Q is is_odd n? *)
+  assert (h := h bot_pval bot_vval val_nil (fun _ => eval_prop bot_pval bot_vval P \/ eval_prop bot_pval bot_vval Q)).
+  edestruct h.
+  - rewrite eval_ren; asimpl; intros; left; auto.
+  - rewrite eval_ren; asimpl; intros; right; auto.
+  - exact 0.
+  - eapply imp_elim; [ apply or_intro1 |].
+    apply reflect0; intro; intros.
+    erewrite closed_eval; eauto.
+  - eapply imp_elim; [apply or_intro2 |].
+    apply reflect1; intro; intros.
+    erewrite closed_eval; eauto.
+Qed.
+
+(* TODO: complete nil P[#n..; ids] -> complete nil ∃ P *)
